Implement 'mem_no_undef_forward_on_storev'

backend/CMinorExperiments.v
@@ -103,6 +103,12 @@ Definition mem_no_undef_fragment (m: mem) : Prop :=
 Definition val_no_pointer (v: val) : Prop :=
   forall bptr i, v <> Vptr bptr i.
 
+
+Definition val_no_undef (v: val) : Prop := v <> Vundef.
+
+Hint Transparent val_no_pointer.
+Hint Transparent val_no_undef.
+
 (* If we have a mem_inj, then we can continue to claim that memory does not
 contain pointers *)
 (* This was so fucking painful, to reason about the case of Get (SetN (encode...)).
@@ -110,6 +116,88 @@ I will probably need to extract that case out *)
 Lemma mem_no_pointers_forward_on_storev:
   forall (m m': mem) (addr v : val),
     val_no_pointer v ->
+    mem_no_pointers m ->
+    Mem.storev STORE_CHUNK_SIZE m addr v = Some m' ->
+    mem_no_pointers m'.
+Proof.
+  intros until v.
+  intros V_NO_POINTER.
+  intros M_NO_POINTERS.
+  intros M'_AS_STORE_M.
+  unfold mem_no_pointers in *.
+  intros until ofs.
+  unfold Mem.storev in M'_AS_STORE_M.
+
+  induction addr; try congruence.
+
+  erewrite Mem.store_mem_contents with (m1 := m)
+                                       (chunk := STORE_CHUNK_SIZE)
+                                       (ofs := (Ptrofs.unsigned i0))
+                                       (b := b0)
+                                       (v := v).
+  assert ({b = b0} + {b <> b0}) as BCASES.
+  apply Pos.eq_dec.
+
+ 
+ destruct BCASES as [BEQ | BNEQ].
+  + subst.
+    rewrite PMap.gss.
+    assert ({ofs = Ptrofs.unsigned i0} +  {ofs <> Ptrofs.unsigned i0}) as
+        ofs_cases.
+    apply Z.eq_dec.
+
+    destruct ofs_cases as [OFSEQ | OFSNEQ].
+    * subst.
+      remember (Ptrofs.unsigned i0) as i0ofs.
+
+      (* we are reading and writing from the same block at the same offset.
+         Convince the damn proof system that we cannot have a fragment by
+       analysing such a load.
+
+       We cannot have a fragment ptr since we same V_NO_PTR*)
+      remember (ZMap.get i0ofs (Mem.setN (encode_val STORE_CHUNK_SIZE v)
+                               i0ofs (Mem.mem_contents m) # b0)) as MNEW.
+
+      assert (ENCODEV: Some MNEW = List.hd_error (encode_val Mint8unsigned v)).
+      rewrite HeqMNEW.
+      erewrite Mem.get_setN_at_base_chunk_Mint8unsigned;
+        try auto;
+        try eassumption.
+
+      induction v;
+        simpl in *;
+        inversion ENCODEV;
+        simpl in *;
+        try congruence.
+
+         unfold inj_bytes.
+         unfold encode_int.
+         unfold rev_if_be.
+         simpl in *.
+         destruct (Archi.big_endian); simpl; congruence.
+      
+    * rewrite Mem.setN_outside.
+      apply M_NO_POINTERS.
+      rewrite encode_val_length.
+      simpl.
+      apply integer_split_number_line.
+      eassumption.
+      
+    
+  + rewrite PMap.gso.
+    apply M_NO_POINTERS.
+    auto.
+
+  + auto.
+Qed.
+
+
+
+(* Note that this proof was the EXACT SAME AS THAT OF
+mem_no_pointer. TODO: CLEAN THIS UP! *)
+Lemma mem_no_undef_forward_on_storev:
+  forall (m m': mem) (addr v : val),
+    val_no_undef v ->
     mem_no_pointers m ->
     Mem.storev STORE_CHUNK_SIZE m addr v = Some m' ->
     mem_no_pointers m'.
@@ -1189,7 +1277,7 @@ Section STMTINTERCHANGE.
         
         eapply memval_inject_trans; try eassumption; try auto.
         eapply mem_no_pointers_forward_on_sseq; try eassumption; try auto.
-        admit. admit.
+        admit.
           
       + (* we're not accessing ARRBLOCK *)
         assert (memval_inject (Mem.flat_inj (Mem.nextblock m))
@@ -1203,11 +1291,20 @@ Section STMTINTERCHANGE.
                               (ZMap.get ofs (Mem.mem_contents m) # b2)
                               (ZMap.get ofs (Mem.mem_contents m21) # b2))
           as MEMVALINJ_m_m21.
+               
         eapply memval_inject_store_no_alias_for_sseq; try auto; try eassumption.
 
+        
+        assert (memval_inject (Mem.flat_inj (Mem.nextblock m))
+                              (ZMap.get ofs (Mem.mem_contents m12) # b2)
+                              (ZMap.get ofs (Mem.mem_contents m) # b2)) as
+            MEMVALINNJ_m12_m.
+        eapply memval_inject_sym;try eassumption; try auto.
 
         
-        
+        eapply memval_inject_trans; try eassumption; try auto.
+        eapply mem_no_pointers_forward_on_sseq; try eassumption; try auto.
+        admit.
   Admitted.
   
   Lemma meminject_ma'_mb': Mem.inject injf m12 m21.
